Splinter/Journal/LikesJournalRefinement.i.dfy
@@ -1,12 +1,12 @@
 include "LikesJournal.i.dfy"
-// include "LinkedJournalRefinement.i.dfy"
+include "LinkedJournalRefinement.i.dfy"
 
 module LikesJournalRefinement {
   import opened Maps
   import opened LSNMod
   import opened LikesJournal
   import LinkedJournal
-//   import LinkedJournalRefinement
+  import LinkedJournalRefinement
 
 
   function IStep(step: Step) : LinkedJournal.Step {
@@ -24,10 +24,101 @@ module LikesJournalRefinement {
 
 // PROVE INVARIANTS
 
+  predicate IndexKeysMapToValidEntries(lsnAddrIndex: map<LSN, Address>, tj: TruncatedJournal)
+    requires tj.WF()
+  {
+    forall lsn | lsn in lsnAddrIndex ::
+      && lsnAddrIndex[lsn] in tj.diskView.entries
+      && tj.diskView.entries[lsnAddrIndex[lsn]].ContainsLSN(lsn)
+  }
+
+  predicate IndexDomainValid(lsnAddrIndex: map<LSN, Address>, tj: TruncatedJournal)
+    requires tj.WF()
+  {
+    // lsnAddrIndex's domain is exactly the set of LSN between journal.SeqStart() and journal.SeqEnd()
+    && (forall lsn :: lsn in lsnAddrIndex <==> tj.SeqStart() <= lsn < tj.SeqEnd())
+  }
+
+  predicate IndexRangeValid(lsnAddrIndex: map<LSN, Address>, tj: TruncatedJournal)
+    requires tj.WF()
+    requires IndexDomainValid(lsnAddrIndex, tj)
+    requires IndexKeysMapToValidEntries(lsnAddrIndex, tj)
+  {
+    forall addr | addr in lsnAddrIndex.Values ::
+      && var msgs := tj.diskView.entries[addr].messageSeq;
+      && var boundaryLSN := tj.diskView.boundaryLSN;
+      && (forall lsn | Mathematics.max(boundaryLSN, msgs.seqStart) <= lsn < msgs.seqEnd :: 
+            && lsn in lsnAddrIndex
+            && lsnAddrIndex[lsn] == addr
+        )
+  }
+
+  // It's not clear we need all these definitions.
+  TransitiveLikes  // functional construction over LinkedJournal
+  FunctionalIndex
+  Index (also imper)
+  ImperativeLikes (imper)
+  
+  // TODO invariant; move to proof
+  predicate ImperativeAgreement(v: Variables) 
+    requires v.WF()
+  {
+    && v.journal.truncatedJournal.diskView.Acyclic()
+    // && v.branchedVars.branched.Valid()
+    && TransitiveLikes(v.journal.truncatedJournal) == ImperativeLikes(v)
+  }
+
+  predicate ImperativeLikesMatchIndex(v: Variables)
+  {
+    ImperativeLikes(v) == multiset(v.lsnAddrIndex.Values)
+  }
+
   predicate Inv(v: Variables)
   {
-    // TODO
-    true
+    var tj :=  v.journal.truncatedJournal;
+    && v.WF()
+    && tj.diskView.Acyclic()
+    && v.lsnAddrIndex == BuildLsnAddrIndex(tj)
+    && v.lsnAddrIndex.Values == tj.Representation() // Our index correctly tracks Linked representation
+    && IndexDomainValid(v.lsnAddrIndex, tj)
+    && IndexKeysMapToValidEntries(v.lsnAddrIndex, tj)
+    && IndexRangeValid(v.lsnAddrIndex, tj)
+    && tj.DiskIsTightWrtRepresentation()
+    && ImperativeLikesMatchIndex(v)
+  }
+  
+  lemma BuildLsnAddrIndexIgnoresBuildTight(dv: DiskView, btRoot: Pointer, root: Pointer)
+    requires dv.Decodable(btRoot)
+    requires dv.Decodable(root)
+    requires dv.Acyclic()
+    requires root.Some? ==> dv.boundaryLSN < dv.entries[root.value].messageSeq.seqEnd
+    requires dv.BuildTight(btRoot).Decodable(root)
+    ensures dv.BuildTight(btRoot).WF()
+    ensures dv.BuildTight(btRoot).Acyclic()
+    ensures root.Some? ==> dv.boundaryLSN < dv.BuildTight(btRoot).entries[root.value].messageSeq.seqEnd
+    ensures BuildLsnAddrIndexDefn(dv, root) == BuildLsnAddrIndexDefn(dv.BuildTight(btRoot), root)
+    decreases dv.TheRankOf(root)
+  {
+    LinkedJournalRefinement.BuildTightIsAwesome(dv, btRoot);
+    if root.Some? {
+      BuildLsnAddrIndexIgnoresBuildTight(dv, btRoot, dv.entries[root.value].CroppedPrior(dv.boundaryLSN));
+    }
+  }
+
+  lemma RepresentationIgnoresBuildTight(dv: DiskView, btRoot: Pointer, root: Pointer)
+    requires dv.Decodable(btRoot)
+    requires dv.Decodable(root)
+    requires dv.Acyclic()
+    requires dv.BuildTight(btRoot).Decodable(root)
+    ensures dv.BuildTight(btRoot).WF()
+    ensures dv.BuildTight(btRoot).Acyclic()
+    ensures dv.BuildTight(btRoot).Representation(root) == dv.Representation(root)
+    decreases dv.TheRankOf(root)
+  {
+    LinkedJournalRefinement.BuildTightIsAwesome(dv, btRoot);
+    if root.Some? {
+      RepresentationIgnoresBuildTight(dv, btRoot, dv.entries[root.value].CroppedPrior(dv.boundaryLSN));
+    }
   }
   
   lemma InvInit(v: Variables, journal: TruncatedJournal)
